src/Arithmetic/MontgomeryReduction/WordByWord/Abstract/Dependent/Definition.v
@@ -1,0 +1,67 @@
+(*** Word-By-Word Montgomery Multiplication *)
+(** This file implements Montgomery Form, Montgomery Reduction, and
+    Montgomery Multiplication on an abstract [T : ℕ → Type].  See
+    https://github.com/mit-plv/fiat-crypto/issues/157 for a discussion
+    of the algorithm; note that it may be that none of the algorithms
+    there exactly match what we're doing here. *)
+Require Import Coq.ZArith.ZArith.
+Require Import Crypto.Util.Notations.
+Require Import Crypto.Util.LetIn.
+
+Local Open Scope Z_scope.
+
+Section WordByWordMontgomery.
+  Local Coercion Z.pos : positive >-> Z.
+  Context
+    {T : nat -> Type}
+    {eval : forall {n}, T n -> Z}
+    {zero : forall {n}, T n}
+    {divmod : forall {n}, T (S n) -> T n * Z} (* returns lowest limb and all-but-lowest-limb *)
+    {r : positive}
+    {R : positive}
+    {R_numlimbs : nat}
+    {scmul : forall {n}, Z -> T n -> T (S n)} (* uses double-output multiply *)
+    {add : forall {n}, T n -> T n -> T (S n)} (* joins carry *)
+    {drop_high : T (S (S R_numlimbs)) -> T (S R_numlimbs)} (* drops the highest limb *)
+    (N : T (S R_numlimbs)).
+
+  (* Recurse for a as many iterations as A has limbs, varying A := A, S := 0, r, bounds *)
+  Section Iteration.
+    Context (pred_A_numlimbs : nat)
+            (B : T R_numlimbs) (k : Z)
+            (A : T (S pred_A_numlimbs))
+            (S : T (S R_numlimbs)).
+    (* Given A, B < R, we want to compute A * B / R mod N. R = bound 0 * ... * bound (n-1) *)
+    Local Definition A_a := dlet p := divmod _ A in p. Local Definition A' := fst A_a. Local Definition a := snd A_a.
+    Local Definition S1 := add _ S (scmul _ a B).
+    Local Definition s := snd (divmod _ S1).
+    Local Definition q := s * k mod r.
+    Local Definition S2 := add _ S1 (scmul _ q N).
+    Local Definition S3 := fst (divmod _ S2).
+    Local Definition S4 := drop_high S3.
+  End Iteration.
+
+  Section loop.
+    Context (A_numlimbs : nat)
+            (A : T A_numlimbs)
+            (B : T R_numlimbs)
+            (k : Z)
+            (S' : T (S R_numlimbs)).
+
+    Definition redc_body {pred_A_numlimbs} : T (S pred_A_numlimbs) * T (S R_numlimbs)
+                                             -> T pred_A_numlimbs * T (S R_numlimbs)
+      := fun '(A, S') => (A' _ A, S4 _ B k A S').
+
+    Fixpoint redc_loop (count : nat) : T count * T (S R_numlimbs) -> T O * T (S R_numlimbs)
+      := match count return T count * _ -> _ with
+         | O => fun A_S => A_S
+         | S count' => fun A_S => redc_loop count' (redc_body A_S)
+         end.
+
+    Definition redc : T (S R_numlimbs)
+      := snd (redc_loop A_numlimbs (A, zero (1 + R_numlimbs))).
+  End loop.
+End WordByWordMontgomery.
+
+Create HintDb word_by_word_montgomery.
+Hint Unfold S4 S3 S2 q s S1 a A' A_a Let_In : word_by_word_montgomery.
